src/3d/Lisp.fsti
@@ -1,14 +1,14 @@
 module Lisp
 open FStar.All
 
-val read_witness_from
-  (from: (unit -> ML string))
-: ML (string & Seq.seq int)
-
 val read_int_from
   (from: (unit -> ML string))
   (name: string)
 : ML (string & int)
+
+val read_bare_int_from
+  (from: (unit -> ML string))
+: ML int
 
 val read_any_from
   (from: (unit -> ML string))
